introduce deletedIdSets

LeanYjs/Algorithm/Basic.lean
@@ -1,2 +1,67 @@
+import LeanYjs.Item
+import Std.Data.ExtTreeSet
+
 inductive IntegrateError where
 | error : IntegrateError
+
+instance : Ord ClientId := inferInstanceAs (Ord Nat)
+instance : Std.TransOrd ClientId := inferInstanceAs (Std.TransOrd Nat)
+instance : Std.LawfulEqOrd ClientId := inferInstanceAs (Std.LawfulEqOrd Nat)
+
+abbrev YjsIdCmp : YjsId → YjsId → Ordering :=
+  compareLex (compareOn YjsId.clientId) (compareOn YjsId.clock)
+
+instance : Std.LawfulEqCmp YjsIdCmp where
+  eq_of_compare := by
+    intro a b h
+    cases a with
+    | mk aClient aClock =>
+      cases b with
+      | mk bClient bClock =>
+        simp [YjsIdCmp, compareLex_eq_eq, compareOn] at h
+        rcases h with ⟨hClient, hClock⟩
+        subst hClient
+        subst hClock
+        rfl
+
+abbrev DeletedIdSet := Std.ExtTreeSet YjsId YjsIdCmp
+
+structure YjsState (A : Type) where
+  items : Array (YjsItem A)
+  deletedIds : DeletedIdSet
+
+instance : Coe (YjsState A) (Array (YjsItem A)) where
+  coe state := state.items
+
+instance : Coe (Array (YjsItem A)) (YjsState A) where
+  coe items := { items := items, deletedIds := ∅ }
+
+@[simp] theorem coeArrayToState_items (items : Array (YjsItem A)) :
+    ((items : YjsState A)).items = items := rfl
+
+@[simp] theorem coeArrayToState_deletedIds (items : Array (YjsItem A)) :
+    ((items : YjsState A)).deletedIds = ∅ := rfl
+
+instance : Coe (Except IntegrateError (YjsState A)) (Except IntegrateError (Array (YjsItem A))) where
+  coe state := state.map YjsState.items
+
+namespace YjsState
+
+def empty : YjsState A := {
+  items := #[]
+  deletedIds := ∅
+}
+
+def toList (state : YjsState A) : List (YjsItem A) :=
+  state.items.toList
+
+def find? (state : YjsState A) (p : YjsItem A → Bool) : Option (YjsItem A) :=
+  state.items.find? p
+
+def addDeletedId (state : YjsState A) (id : YjsId) : YjsState A :=
+  { state with deletedIds := state.deletedIds.insert id }
+
+end YjsState
+
+def YjsEmptyState {A} : YjsState A :=
+  YjsState.empty
