LeanYjs/Order/ItemSetInvariant.lean
@@ -10,23 +10,23 @@ variable {A : Type}
 variable (P : ItemSet A)
 
 structure ItemSetInvariant where
-  origin_not_leq : ∀ (o r : YjsPtr A) c id d, P (YjsItem.mk o r id c d) ->
+  origin_not_leq : ∀ (o r : YjsPtr A) c id, P (YjsItem.mk o r id c) ->
     YjsLt' o r
-  origin_nearest_reachable : ∀ (o r : YjsPtr A) c id d x,
-    P (YjsItem.mk o r id c d) ->
-    OriginReachable (A := A) (YjsItem.mk o r id c d) x ->
+  origin_nearest_reachable : ∀ (o r : YjsPtr A) c id x,
+    P (YjsItem.mk o r id c) ->
+    OriginReachable (A := A) (YjsItem.mk o r id c) x ->
     (YjsLeq' x o) ∨ (YjsLeq' r x)
   id_unique : ∀ (x y : YjsItem A), x.id = y.id -> P x -> P y -> x = y
 
 @[simp] theorem origin_p_valid {A} {P : ItemSet A} : IsClosedItemSet P -> forall (x : YjsItem A), P x -> P x.origin := by
   intros hclosed x px
-  obtain ⟨ o, r, id, c, d ⟩ := x
+  obtain ⟨ o, r, id, c ⟩ := x
   simp at *
   apply hclosed.closedLeft <;> assumption
 
 @[simp] theorem right_origin_p_valid {A} {P : ItemSet A} : IsClosedItemSet P -> forall (x : YjsItem A), P x -> P x.rightOrigin := by
   intros hclosed x px
-  obtain ⟨ o, r, id, c, d ⟩ := x
+  obtain ⟨ o, r, id, c ⟩ := x
   simp at *
   apply hclosed.closedRight <;> assumption
 
@@ -41,7 +41,7 @@ theorem not_ptr_lt_first {A} {P : ItemSet A} : IsClosedItemSet P -> ItemSetInvar
     cases hlt
   | ltOriginOrder o _ hlt =>
     cases hlt
-  | ltRightOrigin h o r id c d hp hlt =>
+  | ltRightOrigin h o r id c hp hlt =>
     cases hlt with
     | leqLt h _ _ hlt =>
       have hsize' : r.size < n := by
@@ -73,7 +73,7 @@ theorem not_last_lt_ptr {A} {P : ItemSet A} : IsClosedItemSet P -> ItemSetInvari
     cases hlt
   | ltOriginOrder _  hpo hlt =>
     cases hlt
-  | ltOrigin h x o r id c d hlt =>
+  | ltOrigin h x o r id c hlt =>
     cases hlt with
     | leqLt h _ _ hlt =>
       have hsize' : o.size < n := by
@@ -129,10 +129,10 @@ theorem ItemSetInvariant.eq_set {A} (P Q : ItemSet A) :
   ItemSetInvariant Q := by
   intros hPclosed hP hiff
   constructor
-  . intros o r c id d hq
+  . intros o r c id hq
     rw [<-hiff] at *
     apply hP.origin_not_leq <;> assumption
-  . intros o r c id d x hq hreachable
+  . intros o r c id x hq hreachable
     rw [<-hiff] at *
     apply hP.origin_nearest_reachable <;> assumption
   . intros x y h_id_eq h_qx h_qy
